Spacetalk/HList.lean
@@ -11,9 +11,9 @@ inductive Member {α : Type u} : α → List α → Type u
   | tail : Member a bs → Member a (b::bs)
 deriving DecidableEq
 
-def List.nth_member : (l : List α) → (n : Fin l.length) → Member (l.get n) l
+def List.nthMember : (l : List α) → (n : Fin l.length) → Member (l.get n) l
   | _::_, ⟨0, _⟩ => .head
-  | _::t, ⟨n'+1, _⟩ => .tail (t.nth_member ⟨n', _⟩)
+  | _::t, ⟨n'+1, _⟩ => .tail (t.nthMember ⟨n', _⟩)
 
 namespace HList
 
@@ -25,9 +25,9 @@ namespace HList
     | a :: as, .head => a
     | _ :: as, .tail h => as.get h
 
-  def get_nth : (l : HList β is) → (n : Fin is.length) → β (is.get n)
+  def getNth : (l : HList β is) → (n : Fin is.length) → β (is.get n)
     | h :: _, ⟨0, _⟩ => h
-    | _ :: t, ⟨n + 1, _⟩ => t.get_nth ⟨n, _⟩
+    | _ :: t, ⟨n + 1, _⟩ => t.getNth ⟨n, _⟩
 
   def append : HList β is1 → HList β is2 → HList β (is1 ++ is2)
     | [], l => l
@@ -40,8 +40,8 @@ end HList
 -- Given a List α, a function f : α → β,
 -- return a HList with indices of type β and values of β-indexed type δ
 -- using the mapping function g : (a : α) → δ (f a).
-def List.to_hlist {α : Type v1} {β : Type v2} {δ : β → Type u}
+def List.toHList {α : Type v1} {β : Type v2} {δ : β → Type u}
                   (f : α → β) (g : (a : α) → δ (f a))
                   : (l : List α) → HList δ (l.map f)
   | [] => []
-  | h :: t => g h :: t.to_hlist f g
+  | h :: t => g h :: t.toHList f g
